little refactor and changes to names, var is splitted to bnode and iri and const is changed to lit

src/Node.v
@@ -3,43 +3,34 @@ From Coq Require Import Strings.String.
 
 Definition eqb_string (x y : string) : bool :=
   if string_dec x y then true else false.
-
+ (* literals should be of Datatype type, is not important for the moment*)
 Inductive node : Type :=
-  | Null
-  | Const (c : nat)
-  | Var (s : string).
+  | Iri (id: string)
+  | Lit (l : nat)
+  | Bnode (name : string).
 
-Definition is_const (n : node) : bool :=
+Definition is_lit (n : node) : bool :=
   (match n with
-   | Const _ => true
+   | Lit _ => true
    | otherwise => false
    end).
 
-Definition is_var (n : node) : bool :=
+Definition is_iri (n : node) : bool :=
   (match n with
-   | Var _ => true
+   | Iri _ => true
    | otherwise => false
    end).
 
-Check (Const 5) : node.
-Check (Var "x") : node.
-Check (Null) : node.
+Definition is_bnode (n : node) : bool :=
+  (match n with
+   | Bnode _ => true
+   | otherwise => false
+   end).
 
 Definition eqb_node (n1 n2 : node) : bool :=
   (match n1, n2 with
-   | (Null), (Null) => true
-   | (Const c1), (Const c2) => c1 =? c2
-   | (Var s1),(Var s2) => eqb s1 s2
+   | (Iri id), (Iri id2) => eqb id id2
+   | (Lit l),(Lit l2) => l =? l2
+   | (Bnode b),(Bnode b2) => eqb b b2
    | e1,e2 => false
    end).
-
-Example eqb_null_node :  eqb_node (Null) (Null) = true.
-Proof. reflexivity. Qed.
-Example eqb_const_eq_node:  eqb_node (Const 5) (Const 5) = true.
-Proof. reflexivity. Qed.
-Example eqb_const_neq_node:  eqb_node (Const 5) (Const 0) = false.
-Proof. reflexivity. Qed.
-Example eqb_var_eq_node :  eqb_node (Var "x") (Var "x") = true.
-Proof. reflexivity. Qed.
-Example eqb_var_neq_node :  eqb_node (Var "x") (Var "y") = false.
-Proof. reflexivity. Qed.
