src/Maps.v
@@ -12,24 +12,24 @@ Definition t_update {A : Type} (m : total_map A)
                     (n : node) (v : A) :=
   fun n' => if eqb_node n n' then v else m n'.
 
-Definition map_const (nod : node) (μ : node -> node) : bool :=
-  (is_const (μ nod)).
+Definition map_lit (nod : node) (μ : node -> node) : bool :=
+  (is_lit (μ nod)).
 
-Definition map_var (nod : node) (μ : node -> node) : bool :=
-  (is_var (μ nod)).
+Definition map_bnode (nod : node) (μ : node -> node) : bool :=
+  (is_bnode (μ nod)).
 
-Definition map_var_or_const (nod : node) (μ : node -> node) : bool :=
-  map_const nod μ || map_var nod μ.
+Definition map_lit_or_bnode (nod : node) (μ : node -> node) : bool :=
+  map_lit nod μ || map_bnode nod μ.
 
 (* want to define this as property of μ given IL B*)
 Definition mapping (IL B : set node) (μ : node -> node) :=
   forall nod : node,
-  (set_In nod IL -> map_const nod μ = true) /\ (set_In nod B -> map_var_or_const nod μ = true).
+  (set_In nod IL -> map_lit nod μ = true) /\ (set_In nod B -> map_lit_or_bnode nod μ = true).
 
 (* want to define this as property of μ given IL B*)
 Definition relabelling (IL B : set node) (μ : node -> node) :=
   forall nod : node,
-  (set_In nod IL -> map_const nod μ = true) /\ (set_In nod B -> map_var nod μ = true).
+  (set_In nod IL -> map_lit nod μ = true) /\ (set_In nod B -> map_bnode nod μ = true).
 
 (*
 Definition mapping (nod : node) (IL B : set node) (μ : node -> node) : bool :=
