src/examples/NodeExamples.v
@@ -1,0 +1,17 @@
+From RDF Require Import Node.
+From Coq Require Import Strings.String.
+
+Check (Lit 5) : node.
+Check (Bnode "b") : node.
+Check (Iri "A") : node.
+
+Example eqb_bnode_ex :  eqb_node (Bnode "b") (Bnode "b") = true.
+Proof. reflexivity. Qed.
+Example eqb_lit_eq_node_ex:  eqb_node (Lit 5) (Lit 5) = true.
+Proof. reflexivity. Qed.
+Example eqb_lit_neq_node:  eqb_node (Lit 5) (Lit 0) = false.
+Proof. reflexivity. Qed.
+Example eqb_iri_eq_node :  eqb_node (Iri "x") (Iri "x") = true.
+Proof. reflexivity. Qed.
+Example eqb_iri_neq_node :  eqb_node (Iri "x") (Iri "y") = false.
+Proof. reflexivity. Qed.
